chore: write correct thm statement

SSA/Experimental/Bits/Fast/MBA.lean
@@ -1,3 +1,8 @@
+@[simp]
+theorem BitVec.zero_concat (b : Bool) : (0#0).concat b = BitVec.ofBool b := by
+  apply BitVec.eq_of_getLsbD_eq
+  simp
+
 namespace MBA
 
 inductive Factor 
@@ -16,25 +21,76 @@ def Factor.denote (w : Nat) (xs : List (BitVec w)) : Factor → BitVec w
 | .xor x y => x.denote w xs &&& y.denote w xs
 | .not x => ~~~ (x.denote w xs)
 
+@[simp]
+theorem Factor.denote_width_zero  (f : Factor) (env : List (BitVec 0)) : 
+   f.denote 0 env = 0#0 := by
+  apply Subsingleton.elim
+
 def Eqn := List (Int × Factor)
 
 def Eqn.denote (e : List (Int × Factor)) 
-    (w : Nat) (env : List (BitVec w)) : BitVec w := 
+    (w : Nat) (env : List (BitVec w)) : Int := 
   match e with
-  | [] => 0#w
-  | (coeff, x) :: xs => coeff * (x.denote w env) + Eqn.denote xs w env 
+  | [] => 0
+  | (coeff, x) :: xs => coeff * (x.denote w env).toInt + Eqn.denote xs w env 
+
+@[simp]
+theorem Eqn.denote_nil  (w : Nat) (env : List (BitVec w)) : 
+    Eqn.denote [] w env = 0 := rfl
+
+@[simp]
+theorem Eqn.denote_cons
+    (coeff : Int) (x : Factor) (es : List (Int × Factor)) (w : Nat) (env : List (BitVec w)) : 
+    Eqn.denote ((coeff, x) :: es) w env = coeff * (x.denote w env).toInt + Eqn.denote es w env := rfl
+
+@[simp]
+theorem Eqn.denote_width_zero  (es : List (Int × Factor)) (env : List (BitVec 0)) : 
+    Eqn.denote es 0 env = 0 := by 
+  induction es 
+  case nil => simp [Eqn.denote]
+  case cons e es ih => 
+    obtain ⟨c, f⟩ := e
+    simp [ih]
+
+/-
+@[simp]
+theorem Eqn.denote_cons'
+    (e : Int × Factor) (es : List (Int × Factor)) (w : Nat) (env : List (BitVec w)) : 
+    Eqn.denote (e :: es) w env = e.1 * (e.2.denote w env) + Eqn.denote es w env := rfl
+
+@[simp]
+theorem Eqn.denote_zero (e : List (Int × Factor)) (env : List (BitVec 0)) : 
+    Eqn.denote e 0 env = 0#0 := by 
+  apply Subsingleton.elim
+-/
 
 theorem Eqn.denote_succ (e : Eqn) (w : Nat) (env : List (BitVec (w + 1))) : 
     Eqn.denote e (w + 1) env = 
-    BitVec.concat (Eqn.denote e w (env.map <| fun x => x.setWidth ..))
-      ((Eqn.denote e 1 (env.map <| fun x => BitVec.ofBool <| x.getLsbD 0)).getLsbD 0) := sorry
+      2 * (Eqn.denote e w (env.map <| fun x => x.extractLsb' 1 w)) +
+      (Eqn.denote e 1 (env.map <| fun x => BitVec.ofBool <| x.getLsbD 0)) := by
+  induction w
+  case zero => 
+    simp
+    induction e 
+    case nil => simp
+    case cons e es ih =>
+      obtain ⟨coeff, f⟩ := e
+      simp
+      rw [← ih]
+      congr
+      suffices heq : (fun x => BitVec.ofBool (x.getLsbD 0)) = id by simp [heq]
+      ext x i hi
+      have : i = 0 := by omega
+      simp [this]
+  case succ w ih =>
+    sorry
+    
 
 theorem Eqn.denote_hard_case (e : Eqn) (h : ∀ (env : List (BitVec 1)), Eqn.denote e 1 env = 0) :
     ∀ (w : Nat) (env : List (BitVec w)), Eqn.denote e w env = 0 := by
   intros w env 
   induction w 
-  case zero =>
-    apply Subsingleton.elim
+  case zero => simp
   case succ w ih =>
     rw [Eqn.denote_succ]
     rw [h]
@@ -49,6 +105,8 @@ theorem Eqn.denote_iff_denote_one (e : Eqn) :
     apply h
   · intros h
     intros w env
+    rw [Eqn.denote_hard_case]
+    exact h
 
 end MBA
 
